src/asn1/ASN1.Spec.Value.SEQUENCE.fst
@@ -7,11 +7,20 @@ open ASN1.Spec.Tag
 open ASN1.Spec.Length
 open ASN1.Spec.Value.Envelop
 
+unfold
+let inbound_sequence_value_of
+  (#k: parser_kind)
+  (#t: Type0)
+  (#p: parser k t)
+  (s: serializer p)
+= inbound_envelop_tag_with_value_of SEQUENCE s
+
 let parse_asn1_sequence_TLV
   (#k: parser_kind)
   (#t: Type0)
   (#p: parser k t)
   (s: serializer p)
+: parser (parse_asn1_envelop_tag_with_TLV_kind SEQUENCE) (inbound_sequence_value_of s)
 = parse_asn1_envelop_tag_with_TLV SEQUENCE s
 
 let serialize_asn1_sequence_TLV
@@ -19,8 +28,16 @@ let serialize_asn1_sequence_TLV
   (#t: Type0)
   (#p: parser k t)
   (s: serializer p)
-: serializer (parse_asn1_envelop_tag_with_TLV SEQUENCE s)
+: serializer (parse_asn1_sequence_TLV s)
 = serialize_asn1_envelop_tag_with_TLV SEQUENCE s
+
+unfold
+let prop_serialize_asn1_sequence_TLV_unfold
+  (#k: parser_kind)
+  (#t: Type0)
+  (#p: parser k t)
+  (s: serializer p)
+= prop_serialize_asn1_envelop_tag_with_TLV_unfold SEQUENCE s
 
 unfold
 let lemma_serialize_asn1_sequence_TLV_unfold
@@ -28,7 +45,17 @@ let lemma_serialize_asn1_sequence_TLV_unfold
   (#t: Type0)
   (#p: parser k t)
   (s: serializer p)
-= lemma_serialize_asn1_envelop_tag_with_TLV_unfold SEQUENCE s
+  (x: inbound_sequence_value_of s)
+: Lemma ( prop_serialize_asn1_sequence_TLV_unfold s x )
+= lemma_serialize_asn1_envelop_tag_with_TLV_unfold SEQUENCE s x
+
+unfold
+let prop_serialize_asn1_sequence_TLV_size
+  (#k: parser_kind)
+  (#t: Type0)
+  (#p: parser k t)
+  (s: serializer p)
+= prop_serialize_asn1_envelop_tag_with_TLV_size SEQUENCE s
 
 unfold
 let lemma_serialize_asn1_sequence_TLV_size
@@ -36,7 +63,9 @@ let lemma_serialize_asn1_sequence_TLV_size
   (#t: Type0)
   (#p: parser k t)
   (s: serializer p)
-= lemma_serialize_asn1_envelop_tag_with_TLV_size SEQUENCE s
+  (x: inbound_sequence_value_of s)
+: Lemma ( prop_serialize_asn1_sequence_TLV_size s x )
+= lemma_serialize_asn1_envelop_tag_with_TLV_size SEQUENCE s x
 
 unfold noextract
 let length_of_asn1_sequence_TLV
@@ -45,11 +74,3 @@ let length_of_asn1_sequence_TLV
   (#p: parser k t)
   (s: serializer p)
 = length_of_asn1_envelop_tag_with_TLV SEQUENCE s
-
-unfold
-let inbound_sequence_value_of
-  (#k: parser_kind)
-  (#t: Type0)
-  (#p: parser k t)
-  (s: serializer p)
-= inbound_envelop_tag_with_value_of SEQUENCE s
