src/asn1/X509.BasicFields.SubjectPublicKeyInfo.fst
@@ -15,18 +15,25 @@ open FStar.Integers
   ======================
 *)
 /// Record repr
-noeq
 type subjectPublicKeyInfo_t
   (alg: cryptoAlg)
 = { subjectPubKey_alg : algorithmIdentifier_t_inbound alg;
-    subjectPubKey     : datatype_of_asn1_type BIT_STRING }
+    subjectPubKey     : pubkey_t alg }
+
+let filter_subjectPublicKeyInfo_t'
+  (alg: cryptoAlg)
+  (x: (algorithmIdentifier_t_inbound alg) `tuple2` (datatype_of_asn1_type BIT_STRING))
+: GTot bool
+= match alg with
+  | ECDSA_P256 -> true
+  | ED25519    -> (snd x).bs_len = 33ul &&
+                  (snd x).bs_unused_bits = 0ul
 
 /// tuple repr
+unfold
 let subjectPublicKeyInfo_t'
   (alg: cryptoAlg)
-= tuple2
-  (algorithmIdentifier_t_inbound alg)
-  (datatype_of_asn1_type BIT_STRING)
+= parse_filter_refine (filter_subjectPublicKeyInfo_t' alg)
 
 let synth_subjectPublicKeyInfo_t
   (alg: cryptoAlg)
@@ -47,6 +54,8 @@ let parse_subjectPublicKeyInfo
 = parse_algorithmIdentifier_sequence_TLV alg
   `nondep_then`
   parse_asn1_TLV_of_type BIT_STRING
+  `parse_filter`
+  filter_subjectPublicKeyInfo_t' alg
   `parse_synth`
   synth_subjectPublicKeyInfo_t alg
 
@@ -56,11 +65,15 @@ let serialize_subjectPublicKeyInfo
 = serialize_synth
   (* p1 *) (parse_algorithmIdentifier_sequence_TLV alg
             `nondep_then`
-            parse_asn1_TLV_of_type BIT_STRING)
+            parse_asn1_TLV_of_type BIT_STRING
+            `parse_filter`
+            filter_subjectPublicKeyInfo_t' alg)
   (* f2 *) (synth_subjectPublicKeyInfo_t alg)
   (* s1 *) (serialize_algorithmIdentifier_sequence_TLV alg
             `serialize_nondep_then`
-            serialize_asn1_TLV_of_type BIT_STRING)
+            serialize_asn1_TLV_of_type BIT_STRING
+            `serialize_filter`
+            filter_subjectPublicKeyInfo_t' alg)
   (* g1 *) (synth_subjectPublicKeyInfo_t' alg)
   (* prf*) ()
 
@@ -80,11 +93,15 @@ let lemma_serialize_subjectPublicKeyInfo_unfold
   serialize_synth_eq
   (* p1 *) (parse_algorithmIdentifier_sequence_TLV alg
             `nondep_then`
-            parse_asn1_TLV_of_type BIT_STRING)
+            parse_asn1_TLV_of_type BIT_STRING
+            `parse_filter`
+            filter_subjectPublicKeyInfo_t' alg)
   (* f2 *) (synth_subjectPublicKeyInfo_t alg)
   (* s1 *) (serialize_algorithmIdentifier_sequence_TLV alg
             `serialize_nondep_then`
-            serialize_asn1_TLV_of_type BIT_STRING)
+            serialize_asn1_TLV_of_type BIT_STRING
+            `serialize_filter`
+            filter_subjectPublicKeyInfo_t' alg)
   (* g1 *) (synth_subjectPublicKeyInfo_t' alg)
   (* prf*) ()
   (* in *) x
@@ -96,13 +113,9 @@ let lemma_serialize_subjectPublicKeyInfo_size
   Seq.length (serialize (serialize_subjectPublicKeyInfo alg) x) ==
   Seq.length (serialize (serialize_algorithmIdentifier_sequence_TLV alg) x.subjectPubKey_alg) +
   Seq.length (serialize (serialize_asn1_TLV_of_type BIT_STRING) x.subjectPubKey)
-  // length_of_opaque_serialization (serialize_subjectPublicKeyInfo alg) x ==
-  // length_of_opaque_serialization (serialize_algorithmIdentifier_sequence_TLV alg) x.subjectPubKey_alg +
-  // length_of_opaque_serialization (serialize_asn1_TLV_of_type BIT_STRING) x.subjectPubKey
 )
 = lemma_serialize_subjectPublicKeyInfo_unfold alg x
 
-(* NOTE: Define the `inbound` version of value type after we defined then serializer. *)
 let subjectPublicKeyInfo_t_inbound
   (alg: cryptoAlg)
 = inbound_sequence_value_of (serialize_subjectPublicKeyInfo alg)
@@ -121,11 +134,32 @@ let serialize_subjectPublicKeyInfo_sequence_TLV
 
 let lemma_serialize_subjectPublicKeyInfo_sequence_TLV_unfold
   (alg: cryptoAlg)
-= lemma_serialize_asn1_sequence_TLV_unfold (serialize_subjectPublicKeyInfo alg)
+  (x: subjectPublicKeyInfo_t_inbound alg)
+: Lemma ( prop_serialize_asn1_sequence_TLV_unfold (serialize_subjectPublicKeyInfo alg) x )
+= lemma_serialize_asn1_sequence_TLV_unfold (serialize_subjectPublicKeyInfo alg) x
 
 let lemma_serialize_subjectPublicKeyInfo_sequence_TLV_size
   (alg: cryptoAlg)
-= lemma_serialize_asn1_sequence_TLV_size (serialize_subjectPublicKeyInfo alg)
+  (x: subjectPublicKeyInfo_t_inbound alg)
+: Lemma ( prop_serialize_asn1_sequence_TLV_size (serialize_subjectPublicKeyInfo alg) x )
+= lemma_serialize_asn1_sequence_TLV_size (serialize_subjectPublicKeyInfo alg) x
+
+let lemma_serialize_subjectPublicKeyInfo_sequence_TLV_size_exact
+  (alg: cryptoAlg {alg == ED25519})
+  (x: subjectPublicKeyInfo_t_inbound alg)
+: Lemma (
+  match alg with
+  | ED25519   -> ( length_of_opaque_serialization (serialize_subjectPublicKeyInfo_sequence_TLV alg) x == 44 )
+)
+= admit()
+  // match alg with
+  // | ED25519   -> ( lemma_serialize_subjectPublicKeyInfo_sequence_TLV_unfold alg x;
+  //                  lemma_serialize_subjectPublicKeyInfo_sequence_TLV_size   alg x;
+  //                    lemma_serialize_subjectPublicKeyInfo_size alg x;
+  //                    (**) lemma_serialize_algorithmIdentifier_sequence_TLV_size_exact alg x.subjectPubKey_alg;
+  //                  // assume ( let bs: pubkey_t ED25519 = x.subjectPubKey in
+  //                  //          length_of_asn1_primitive_TLV bs == 35 );
+  //                  admit() )
 
 /// Low
 ///
@@ -137,7 +171,9 @@ let serialize32_subjectPublicKeyInfo_backwards
 = serialize32_synth_backwards
   (* ls *) (serialize32_algorithmIdentifier_sequence_TLV_backwards alg
             `serialize32_nondep_then_backwards`
-            serialize32_asn1_TLV_backwards_of_type BIT_STRING)
+            serialize32_asn1_TLV_backwards_of_type BIT_STRING
+            `serialize32_filter_backwards`
+            filter_subjectPublicKeyInfo_t' alg)
   (* f2 *) (synth_subjectPublicKeyInfo_t alg)
   (* g1 *) (synth_subjectPublicKeyInfo_t' alg)
   (* g1'*) (synth_subjectPublicKeyInfo_t' alg)
