src/asn1/X509.Crypto.Signature.fst
@@ -10,9 +10,71 @@ open X509.Base
 
 open FStar.Integers
 module B32 = FStar.Bytes
-(*)
-noeq
-type x509_signature_ECDSA_P256_t = {
-  r: 
-  s:
-  }
+
+open ASN1.Base
+
+let x509_signature_t
+  (alg: cryptoAlg {alg == ED25519})
+= match alg with
+  | ED25519   -> datatype_of_asn1_type BIT_STRING
+
+let parse_x509_signature_kind
+  (alg: cryptoAlg {alg == ED25519})
+= match alg with
+  | ED25519   -> parse_asn1_TLV_kind_of_type BIT_STRING
+
+let parse_x509_signature
+  (alg: cryptoAlg {alg == ED25519})
+: parser (parse_x509_signature_kind alg) (x509_signature_t alg)
+= match alg with
+  | ED25519   -> ( parse_asn1_TLV_of_type BIT_STRING )
+
+let serialize_x509_signature
+  (alg: cryptoAlg {alg == ED25519})
+: serializer (parse_x509_signature alg)
+= match alg with
+  | ED25519   -> ( serialize_asn1_TLV_of_type BIT_STRING )
+
+let x509_signature_t_inbound
+  (alg: cryptoAlg {alg == ED25519})
+= match alg with
+  | ED25519   -> ( inbound_sequence_value_of (serialize_x509_signature alg) )
+
+let parse_x509_signature_sequence_TLV
+  (alg: cryptoAlg {alg == ED25519})
+: parser _ (x509_signature_t_inbound alg)
+= match alg with
+  | ED25519   -> ( parse_asn1_sequence_TLV (serialize_x509_signature alg) )
+
+let serialize_x509_signature_sequence_TLV
+  (alg: cryptoAlg {alg == ED25519})
+: serializer (parse_x509_signature_sequence_TLV alg)
+= match alg with
+  | ED25519   -> ( serialize_asn1_sequence_TLV (serialize_x509_signature alg) )
+
+let lemma_serialize_x509_signature_sequence_TLV_unfold
+  (alg: cryptoAlg {alg == ED25519})
+  (x: x509_signature_t_inbound alg)
+: Lemma ( prop_serialize_asn1_sequence_TLV_unfold (serialize_x509_signature alg) x )
+= match alg with
+  | ED25519   -> ( lemma_serialize_asn1_sequence_TLV_unfold (serialize_x509_signature alg) x )
+
+let lemma_serialize_x509_signature_sequence_TLV_size
+  (alg: cryptoAlg {alg == ED25519})
+  (x: x509_signature_t_inbound alg)
+: Lemma ( prop_serialize_asn1_sequence_TLV_size (serialize_x509_signature alg) x )
+= match alg with
+  | ED25519   -> ( lemma_serialize_asn1_sequence_TLV_size (serialize_x509_signature alg) x )
+
+(* Low *)
+let serialize32_x509_signature_backwards
+  (alg: cryptoAlg {alg == ED25519})
+: serializer32_backwards (serialize_x509_signature alg)
+= match alg with
+  | ED25519   -> ( serialize32_asn1_bit_string_TLV_backwards () )
+
+let serialize32_x509_signature_sequence_TLV_backwards
+  (alg: cryptoAlg {alg == ED25519})
+: serializer32_backwards (serialize_x509_signature_sequence_TLV alg)
+= match alg with
+  | ED25519   -> ( serialize32_asn1_sequence_TLV_backwards (serialize32_x509_signature_backwards alg) )
