src/asn1/RIoT.X509.Base.fst
@@ -1,5 +1,5 @@
 module RIoT.X509.Base
 open X509.Base
 
-let alg_DeviceID = ECDSA_P256
-let alg_AliasKey = ECDSA_P256
+let alg_DeviceID = ED25519
+let alg_AliasKey = ED25519
