src/asn1/RIoT.X509.fst
@@ -16,19 +16,18 @@ let _ = assert (length_of_asn1_primitive_TLV (Mkbit_string_t 33ul 0ul (magic()))
 
 #push-options "--query_stats --z3rlimit 16 --initial_fuel 2 --initial_ifuel 1"
 let x509_get_public_key_info
-  (pubkey_alg: cryptoAlg)
-  (pubkey: pubkey_t pubkey_alg)
+  (pubkey_alg: cryptoAlg {pubkey_alg == ED25519} )
+  (pubkey: B32.lbytes32 32ul)
 : Tot (subjectPublicKeyInfo_t_inbound pubkey_alg)
-= let pubkey_bs: datatype_of_asn1_type BIT_STRING = Mkbit_string_t 33ul 0ul pubkey in
-  if (pubkey_alg = ECDSA_P256) then
-  ( let alg_id: algorithmIdentifier_t pubkey_alg = {  // 1 + 1 + (7 + 8) = 17
-       alg_id_oid_ecdsa = OID_EC_ALG_UNRESTRICTED;    // 1 + 1 + 5 = 7
-       alg_id_oid_p256  = OID_EC_GRP_SECP256R1        // 1 + 1 + 6 = 8
+= let pubkey_bs: pubkey_t pubkey_alg = Mkbit_string_t 33ul 0ul pubkey in
+  if (pubkey_alg = ED25519) then
+  ( let alg_id: algorithmIdentifier_t pubkey_alg = {
+       algID_ed25519 = OID_ED25519
     } in
     (* Prf *) lemma_serialize_algorithmIdentifier_unfold pubkey_alg alg_id;
-    (* Prf *) lemma_serialize_asn1_oid_TLV_size alg_id.alg_id_oid_ecdsa;
-    (* Prf *) lemma_serialize_asn1_oid_TLV_size alg_id.alg_id_oid_p256;
-    (* Prf *) lemma_serialize_algorithmIdentifier_sequence_TLV_size pubkey_alg alg_id;
+    (* Prf *) lemma_serialize_asn1_oid_TLV_size alg_id.algID_ed25519;
+    // (* Prf *) lemma_serialize_algorithmIdentifier_sequence_TLV_size pubkey_alg alg_id;
+    (* Prf *) lemma_serialize_algorithmIdentifier_sequence_TLV_size_exact pubkey_alg alg_id;
 
     let aliasPublicKeyInfo: subjectPublicKeyInfo_t pubkey_alg = {// 1 + 1 + (17 + 35) = 54
        subjectPubKey_alg = alg_id;                             // 17
@@ -37,28 +36,30 @@ let x509_get_public_key_info
   (* Prf *) lemma_serialize_subjectPublicKeyInfo_unfold pubkey_alg aliasPublicKeyInfo;
   (* Prf *) lemma_serialize_subjectPublicKeyInfo_size pubkey_alg aliasPublicKeyInfo;
   (* Prf *) lemma_serialize_asn1_bit_string_TLV_size aliasPublicKeyInfo.subjectPubKey;
-  (* Prf *) lemma_serialize_subjectPublicKeyInfo_sequence_TLV_size pubkey_alg aliasPublicKeyInfo;
+  // (* Prf *) lemma_serialize_subjectPublicKeyInfo_sequence_TLV_size pubkey_alg aliasPublicKeyInfo;
+  (* Prf *) lemma_serialize_subjectPublicKeyInfo_sequence_TLV_size_exact pubkey_alg aliasPublicKeyInfo;
 
   (* return *) aliasPublicKeyInfo )
   else
   ( false_elim() )
 #pop-options
 
-#push-options "--query_stats --z3rlimit 96 --initial_fuel 16 --max_fuel 32 --initial_ifuel 2"
-let x509_get_compositeDeviceID
+#push-options "--query_stats --z3rlimit 192 --initial_fuel 16 --max_fuel 32 --initial_ifuel 2"
+let x509_get_riot_extension
   (version: datatype_of_asn1_type INTEGER)
   (deviceKeyPub: B32.lbytes32 32ul)
   (fwid: B32.lbytes32 32ul)
-: Tot (compositeDeviceID_t_inbound)
+: Tot (x509_extension_t_inbound serialize_compositeDeviceID_sequence_TLV)
 = let deviceIDPublicKeyInfo: subjectPublicKeyInfo_t alg_DeviceID = x509_get_public_key_info alg_DeviceID deviceKeyPub in
-  (* Prf *) lemma_serialize_subjectPublicKeyInfo_unfold alg_DeviceID deviceIDPublicKeyInfo;
-  (* Prf *) lemma_serialize_subjectPublicKeyInfo_size alg_DeviceID deviceIDPublicKeyInfo;
-  (* Prf *)      lemma_serialize_algorithmIdentifier_unfold alg_DeviceID deviceIDPublicKeyInfo.subjectPubKey_alg;
-  (* Prf *)      (**) lemma_serialize_asn1_oid_TLV_size deviceIDPublicKeyInfo.subjectPubKey_alg.alg_id_oid_ecdsa;
-  (* Prf *)      (**) lemma_serialize_asn1_oid_TLV_size deviceIDPublicKeyInfo.subjectPubKey_alg.alg_id_oid_p256;
-  (* Prf *)      lemma_serialize_algorithmIdentifier_sequence_TLV_size alg_DeviceID deviceIDPublicKeyInfo.subjectPubKey_alg;
-  (* Prf *) (**) lemma_serialize_asn1_bit_string_TLV_size deviceIDPublicKeyInfo.subjectPubKey;
-  (* Prf *) lemma_serialize_subjectPublicKeyInfo_sequence_TLV_size alg_DeviceID deviceIDPublicKeyInfo;
+  // (* Prf *) lemma_serialize_subjectPublicKeyInfo_unfold alg_DeviceID deviceIDPublicKeyInfo;
+  // (* Prf *) lemma_serialize_subjectPublicKeyInfo_size alg_DeviceID deviceIDPublicKeyInfo;
+  // (* Prf *)      lemma_serialize_algorithmIdentifier_unfold alg_DeviceID deviceIDPublicKeyInfo.subjectPubKey_alg;
+  // (* Prf *)      (**) lemma_serialize_asn1_oid_TLV_size deviceIDPublicKeyInfo.subjectPubKey_alg.algID_ed25519;
+  // (* Prf *)      lemma_serialize_algorithmIdentifier_sequence_TLV_size alg_DeviceID deviceIDPublicKeyInfo.subjectPubKey_alg;
+  // (* Prf *)      lemma_serialize_algorithmIdentifier_sequence_TLV_size_exact alg_DeviceID deviceIDPublicKeyInfo.subjectPubKey_alg;
+  // (* Prf *) (**) lemma_serialize_asn1_bit_string_TLV_size deviceIDPublicKeyInfo.subjectPubKey;
+  // (* Prf *) lemma_serialize_subjectPublicKeyInfo_sequence_TLV_size alg_DeviceID deviceIDPublicKeyInfo;
+  (* Prf *) lemma_serialize_subjectPublicKeyInfo_sequence_TLV_size_exact alg_DeviceID deviceIDPublicKeyInfo;
 
   let fwid: fwid_t = {
     fwid_hashAlg = OID_DIGEST_SHA256;
@@ -68,6 +69,7 @@ let x509_get_compositeDeviceID
   (* Prf *) (**) lemma_serialize_asn1_oid_TLV_size fwid.fwid_hashAlg;
   (* Prf *) (**) lemma_serialize_asn1_octet_string_TLV_size fwid.fwid_value;
   (* Prf *) lemma_serialize_fwid_sequence_TLV_size fwid;
+  (* Prf *) lemma_serialize_fwid_sequence_TLV_size_exact fwid;
 
   let compositeDeviceID: compositeDeviceID_t = {
     riot_version  = version;
@@ -77,14 +79,90 @@ let x509_get_compositeDeviceID
   (* Prf *) lemma_serialize_compositeDeviceID_size compositeDeviceID;
   (* Prf *) (**) lemma_serialize_asn1_integer_TLV_size compositeDeviceID.riot_version;
   (* Prf *) lemma_serialize_compositeDeviceID_sequence_TLV_size compositeDeviceID;
+  (* Prf *) lemma_serialize_compositeDeviceID_sequence_TLV_size_exact compositeDeviceID;
 
-(*return*) compositeDeviceID
+  let riot_extension: x509_extension_t serialize_compositeDeviceID_sequence_TLV = {
+    x509_extID       = OID_RIOT;
+    x509_extCritical = false;
+    x509_extValue    = compositeDeviceID
+  } in
+  (* Prf *) lemma_serialize_x509_extension_unfold
+            (* s *) serialize_compositeDeviceID_sequence_TLV
+            (* x *) riot_extension;
+  (* Prf *) lemma_serialize_x509_extension_size
+            (* s *) serialize_compositeDeviceID_sequence_TLV
+            (* x *) riot_extension;
+  (* Prf *) (**) lemma_serialize_asn1_oid_TLV_size riot_extension.x509_extID;
+  (* Prf *) (**) lemma_serialize_asn1_boolean_TLV_size riot_extension.x509_extCritical;
+  // assert_norm (length_of_asn1_primitive_TLV riot_extension.x509_extID == 11);
+  // assert_norm (length_of_asn1_primitive_TLV riot_extension.x509_extCritical == 3);
+  // assert_norm (length_of_asn1_primitive_TLV riot_extension.x509_extValue.riot_version <= 6);
+  // assert_norm (length_of_opaque_serialization serialize_fwid_sequence_TLV riot_extension.x509_extValue.riot_fwid == 47);
+  (* Prf *) lemma_serialize_x509_extension_sequence_TLV_size
+            (* s *) serialize_compositeDeviceID_sequence_TLV
+            (* x *) riot_extension;
+
+(*return*) riot_extension
 #pop-options
 
-(* TODO)
-let _ = assert (length_of_oid OID_EC_GRP_SECP256R1 == 6)
-let _ = assert (length_of_asn1_primitive_TLV (Mkbit_string_t 33ul 0ul (magic())) == 35)
+open Lib.IntTypes
+open RIoT.Base
+open RIoT.Declassify
+open Spec.Hash.Definitions
 
+let bytes_pub  = Seq.seq pub_uint8
+let lbytes_pub = Seq.lseq pub_uint8
+let bytes_sec  = Seq.seq uint8
+let lbytes_sec = Seq.lseq uint8
+
+
+#restart-solver
+#push-options "--query_stats --z3rlimit 256 --initial_fuel 8 --initial_ifuel 3"
+let x509_get_aliasKey_crt_tbs_spec
+  (cdi: lbytes_sec 32)
+  (fwid: lbytes_sec 32)
+  (riot_ver: datatype_of_asn1_type INTEGER)
+  (riot_label_DeviceID_len: size_t { (* for Hacl.HKDF.expand_st *)
+                                     hash_length alg + v riot_label_DeviceID_len + 1 + block_length alg < pow2 32 /\
+                                     (* for Spec.Aigle.HKDF.expand *)
+                                     hash_length alg + v riot_label_DeviceID_len + 1 + block_length alg < max_input_length alg })
+  (riot_label_DeviceID: lbytes_sec (v riot_label_DeviceID_len))
+  (aliasKey_crt_len: size_t)
+  (aliasKey_crt_pos: size_t { 0 <= v aliasKey_crt_pos /\
+                              v aliasKey_crt_pos <= v aliasKey_crt_len })
+  (aliasKey_crt: lbytes_pub (v aliasKey_crt_len))
+// : GTot (l: nat & lbytes_pub l)
+= let cdigest = Spec.Agile.Hash.hash alg cdi in
+  let deviceID_pub, deviceID_priv = riot_derive_key_pair_spec
+                                    (* ikm *) 32ul cdigest
+                                    (* lbl *) riot_label_DeviceID_len riot_label_DeviceID in
+  let adigest = Spec.Agile.HMAC.hmac alg cdigest fwid in
+  let aliasKey_pub, aliasKey_priv = riot_derive_key_pair_spec
+                                    (* ikm *) 32ul adigest
+                                    (* lbl *) riot_label_DeviceID_len riot_label_DeviceID in
+  let deviceID_pub32: B32.lbytes32 32ul = B32.hide deviceID_pub in
+  let fwid32: B32.lbytes32 32ul = B32.hide (declassify_secret_bytes 32 fwid) in
+  let riot_extension = x509_get_riot_extension riot_ver deviceID_pub32 fwid32 in
+  let riot_extension_sx = serialize_x509_extension_sequence_TLV serialize_compositeDeviceID_sequence_TLV
+                          `serialize`
+                          riot_extension in
+  (* AliasKey Certificate TBS *)
+  let aliasKey_crt_tbs = Seq.slice aliasKey_crt 0 (v aliasKey_crt_pos)
+                         `Seq.append` (* FIXME: Here, we need to require that `tbs`'s length is acceptable by the signing func *)
+                         riot_extension_sx in
+  // let _ = lemma_serialize_x509_extension_size serialize_compositeDeviceID_sequence_TLV riot_extension;
+  //         (**) lemma_serialize_asn1_oid_TLV_size riot_extension.x509_extID;
+  //         (**) lemma_serialize_asn1_boolean_TLV_size riot_extension.x509_extCritical;
+  //         (**) lemma_serialize_compositeDeviceID_sequence_TLV_size_exact riot_extension.x509_extValue;
+  //         lemma_serialize_x509_extension_sequence_TLV_size serialize_compositeDeviceID_sequence_TLV riot_extension in
+  // let aliasKey_crt_tbs = classify_public_bytes (Seq.length aliasKey_crt_tbs) aliasKey_crt_tbs in
+
+(* return *) (|Seq.length aliasKey_crt_tbs, aliasKey_crt_tbs|)
+
+// let _ = assert (length_of_oid OID_EC_GRP_SECP256R1 == 6)
+// let _ = assert (length_of_asn1_primitive_TLV (Mkbit_string_t 33ul 0ul (magic())) == 35)
+
+(*
 #push-options "--query_stats --z3rlimit 96 --initial_fuel 16 --max_fuel 32 --initial_ifuel 2"
 let x509_get_riot_extension
   (version: datatype_of_asn1_type INTEGER)
