src/asn1/X509.Base.fst
@@ -12,15 +12,20 @@ module B32 = FStar.Bytes
 
 type cryptoAlg =
 | ECDSA_P256
+| ED25519
 
 unfold
 let pubkey_len
   (pubkey_alg: cryptoAlg)
 = match pubkey_alg with
   | ECDSA_P256 -> 32ul
+  | ED25519    -> 32ul
 
 unfold
 let pubkey_t
   (pubkey_alg: cryptoAlg)
 = match pubkey_alg with
-  | ECDSA_P256 -> B32.lbytes32 (pubkey_len pubkey_alg)
+  | ECDSA_P256 -> datatype_of_asn1_type BIT_STRING
+  | ED25519    -> bs: datatype_of_asn1_type BIT_STRING
+                     { bs.bs_len == 33ul /\
+                       bs.bs_unused_bits == 0ul}
