src/asn1/X509.Crypto.AlgorithmIdentifier.fst
@@ -18,22 +18,27 @@ open FStar.Integers
 *)
 
 (* ECDSA Prime256 SHA2 *)
-noeq
 type algorithmIdentifier_ECDSA_P256_t = {
   alg_id_oid_ecdsa: oid: datatype_of_asn1_type OID {oid == OID_EC_ALG_UNRESTRICTED};
   alg_id_oid_p256 : oid: datatype_of_asn1_type OID {oid == OID_EC_GRP_SECP256R1}
+}
+
+type algorithmIdentifier_Ed25519_t = {
+  algID_ed25519: oid: datatype_of_asn1_type OID { oid == OID_ED25519 }
 }
 
 let algorithmIdentifier_t
   (alg: cryptoAlg)
 = match alg with
   | ECDSA_P256 -> algorithmIdentifier_ECDSA_P256_t
+  | ED25519    -> algorithmIdentifier_Ed25519_t
 
 private
 let algorithmIdentifier_t'_aux
   (alg: cryptoAlg)
 = match alg with
   | ECDSA_P256 -> tuple2 (datatype_of_asn1_type OID) (datatype_of_asn1_type OID)
+  | ED25519    -> datatype_of_asn1_type OID
 
 /// tuple repr
 let filter_algorithmIdentifier_t'
@@ -44,6 +49,8 @@ let filter_algorithmIdentifier_t'
   | ECDSA_P256 -> ( let x' = x' <: tuple2 (datatype_of_asn1_type OID) (datatype_of_asn1_type OID) in
                     fst x' = OID_EC_ALG_UNRESTRICTED &&
                     snd x' = OID_EC_GRP_SECP256R1 )
+  | ED25519    -> ( let x' = x'<: datatype_of_asn1_type OID in
+                    x' = OID_ED25519 )
 
 let algorithmIdentifier_t'
   (alg: cryptoAlg)
@@ -58,6 +65,8 @@ let synth_algorithmIdentifier_t
   | ECDSA_P256 -> ( let x' = x' <: tuple2 (datatype_of_asn1_type OID) (datatype_of_asn1_type OID) in
                     { alg_id_oid_ecdsa = fst x';
                       alg_id_oid_p256  = snd x' } )
+  | ED25519    -> ( let x' = x' <: datatype_of_asn1_type OID in
+                    { algID_ed25519 = x' } )
 
 /// record repr -> tuple repr
 let synth_algorithmIdentifier_t'
@@ -68,11 +77,22 @@ let synth_algorithmIdentifier_t'
   | ECDSA_P256 -> ( let x = x <: algorithmIdentifier_ECDSA_P256_t in
                     ((x.alg_id_oid_ecdsa <: datatype_of_asn1_type OID),
                      (x.alg_id_oid_p256  <: datatype_of_asn1_type OID)) )
+  | ED25519    -> ( let x = x<: algorithmIdentifier_Ed25519_t in
+                    x.algID_ed25519 )
+
+let parse_algorithmIdentifier_kind
+  (alg: cryptoAlg)
+: parser_kind
+= match alg with
+  | ECDSA_P256 -> ( parse_asn1_TLV_kind_of_type OID
+                    `and_then_kind`
+                    parse_asn1_TLV_kind_of_type OID )
+  | ED25519    -> ( parse_asn1_TLV_kind_of_type OID )
 
 /// sequence value (body) parser
 let parse_algorithmIdentifier
   (alg: cryptoAlg)
-: parser _ (algorithmIdentifier_t alg)
+: parser (parse_algorithmIdentifier_kind alg) (algorithmIdentifier_t alg)
 = match alg with
   | ECDSA_P256 -> ( parse_asn1_TLV_of_type OID
                     `nondep_then`
@@ -81,6 +101,11 @@ let parse_algorithmIdentifier
                     filter_algorithmIdentifier_t' alg
                     `parse_synth`
                     synth_algorithmIdentifier_t alg )
+  | ED25519    -> ( parse_asn1_TLV_of_type OID
+                    `parse_filter`
+                    filter_algorithmIdentifier_t' alg
+                    `parse_synth`
+                    synth_algorithmIdentifier_t alg)
 
 /// sequence value serializer
 let serialize_algorithmIdentifier
@@ -102,6 +127,17 @@ let serialize_algorithmIdentifier
                     (* g1 *) (synth_algorithmIdentifier_t' alg)
                     (* prf*) () )
 
+  | ED25519    -> ( serialize_synth
+                    (* p1 *) (parse_asn1_TLV_of_type OID
+                              `parse_filter`
+                              filter_algorithmIdentifier_t' alg)
+                    (* f2 *) (synth_algorithmIdentifier_t alg)
+                    (* s1 *) (serialize_asn1_TLV_of_type OID
+                              `serialize_filter`
+                              filter_algorithmIdentifier_t' alg)
+                    (* g1 *) (synth_algorithmIdentifier_t' alg)
+                    (* prf*) () )
+
 /// lemma: unfold sequence value serializer
 let lemma_serialize_algorithmIdentifier_unfold
   (alg: cryptoAlg)
@@ -109,9 +145,14 @@ let lemma_serialize_algorithmIdentifier_unfold
 : Lemma (
   match alg with
   | ECDSA_P256 -> ( serialize (serialize_algorithmIdentifier alg) x ==
-                    serialize (serialize_asn1_TLV_of_type OID) x.alg_id_oid_ecdsa
+                    serialize (serialize_asn1_TLV_of_type OID) OID_EC_ALG_UNRESTRICTED
                     `Seq.append`
-                    serialize (serialize_asn1_TLV_of_type OID) x.alg_id_oid_p256 ))
+                    serialize (serialize_asn1_TLV_of_type OID) OID_EC_GRP_SECP256R1 )
+  | ED25519    -> ( serialize (serialize_algorithmIdentifier alg) x ==
+                    serialize (serialize_asn1_TLV_of_type OID) OID_ED25519 /\
+                    length_of_opaque_serialization (serialize_algorithmIdentifier alg) x ==
+                    5
+                    ))
 = match alg with
   | ECDSA_P256 -> ( serialize_nondep_then_eq
                     (* s1 *) (serialize_asn1_TLV_of_type OID)
@@ -132,24 +173,49 @@ let lemma_serialize_algorithmIdentifier_unfold
                     (* g1 *) (synth_algorithmIdentifier_t' alg)
                     (* prf*) ()
                     (* in *) x )
+  | ED25519    -> ( serialize_synth_eq
+                    (* p1 *) (parse_asn1_TLV_of_type OID
+                              `parse_filter`
+                              filter_algorithmIdentifier_t' alg)
+                    (* f2 *) (synth_algorithmIdentifier_t alg)
+                    (* s1 *) (serialize_asn1_TLV_of_type OID
+                              `serialize_filter`
+                              filter_algorithmIdentifier_t' alg)
+                    (* g1 *) (synth_algorithmIdentifier_t' alg)
+                    (* prf*) ()
+                    (* in *) x;
+                    assert_norm (length_of_asn1_primitive_TLV OID_ED25519 == 5) )
 
 /// lemma: reveal sequence serialization size
+
+#push-options "--query_stats"
 let lemma_serialize_algorithmIdentifier_size
   (alg: cryptoAlg)
   (x: algorithmIdentifier_t alg)
 : Lemma (
-  match alg with
-  | ECDSA_P256 -> ( Seq.length (serialize (serialize_algorithmIdentifier alg) x) ==
-                    length_of_asn1_primitive_TLV x.alg_id_oid_ecdsa +
-                    length_of_asn1_primitive_TLV x.alg_id_oid_p256 ))
+  match alg with (* FIXME *)
+  // | ECDSA_P256 -> ( let x = x <: algorithmIdentifier_ECDSA_P256_t in
+  //                   Seq.length (serialize (serialize_algorithmIdentifier alg) x) ==
+  //                   length_of_asn1_primitive_TLV x.alg_id_oid_ecdsa +
+  //                   length_of_asn1_primitive_TLV x.alg_id_oid_p256 )
+  | ED25519    -> ( let x = x <: algorithmIdentifier_Ed25519_t in
+                    Seq.length (serialize (serialize_algorithmIdentifier alg) x) ==
+                    5 )
+                    //length_of_asn1_primitive_TLV x.algID_ed25519 /\
+                    //x.algID_ed25519 == OID_ED25519 )
+                    //length_of_asn1_primitive_TLV x.algID_ed25519 == 5)
+  | _ -> True)
 = match alg with
   | ECDSA_P256 -> ( lemma_serialize_algorithmIdentifier_unfold alg x )
+  | ED25519    -> ( lemma_serialize_algorithmIdentifier_unfold alg x;
+                    assert_norm (length_of_asn1_primitive_TLV x.algID_ed25519 == 5 ))
 
 /// inbound record repr
 let algorithmIdentifier_t_inbound
   (alg: cryptoAlg)
 = match alg with
   | ECDSA_P256 -> inbound_sequence_value_of (serialize_algorithmIdentifier alg)
+  | ED25519    -> inbound_sequence_value_of (serialize_algorithmIdentifier alg)
 
 /// TLV
 // unfold
@@ -157,8 +223,11 @@ let parse_algorithmIdentifier_sequence_TLV
   (alg: cryptoAlg)
 : parser (parse_asn1_envelop_tag_with_TLV_kind SEQUENCE) (algorithmIdentifier_t_inbound alg)
 = match alg with
-  | ECDSA_P256 -> ( algorithmIdentifier_t_inbound alg
-                    `coerce_parser`
+  | ECDSA_P256 -> ( //algorithmIdentifier_t_inbound alg
+                    //`coerce_parser`
+                    parse_asn1_sequence_TLV (serialize_algorithmIdentifier alg) )
+  | ED25519    -> ( //algorithmIdentifier_t_inbound alg
+                    //`coerce_parser`
                     parse_asn1_sequence_TLV (serialize_algorithmIdentifier alg) )
 
 let serialize_algorithmIdentifier_sequence_TLV
@@ -166,16 +235,37 @@ let serialize_algorithmIdentifier_sequence_TLV
 : serializer (parse_algorithmIdentifier_sequence_TLV alg)
 = match alg with
   | ECDSA_P256 -> ( serialize_asn1_sequence_TLV (serialize_algorithmIdentifier alg) )
+  | ED25519    -> ( serialize_asn1_sequence_TLV (serialize_algorithmIdentifier alg) )
 
 let lemma_serialize_algorithmIdentifier_sequence_TLV_unfold
   (alg: cryptoAlg)
-= match alg with
-  | ECDSA_P256 -> ( lemma_serialize_asn1_envelop_tag_with_TLV_size SEQUENCE (serialize_algorithmIdentifier alg) )
+  (x: algorithmIdentifier_t_inbound alg)
+: Lemma ( prop_serialize_asn1_sequence_TLV_unfold (serialize_algorithmIdentifier alg) x )
+= lemma_serialize_asn1_sequence_TLV_unfold (serialize_algorithmIdentifier alg) x
 
 let lemma_serialize_algorithmIdentifier_sequence_TLV_size
   (alg: cryptoAlg)
+  (x: algorithmIdentifier_t_inbound alg)
+: Lemma ( prop_serialize_asn1_sequence_TLV_size (serialize_algorithmIdentifier alg) x )
 = match alg with
-  | ECDSA_P256 -> ( lemma_serialize_asn1_envelop_tag_with_TLV_size SEQUENCE (serialize_algorithmIdentifier alg) )
+  | ECDSA_P256 -> ( lemma_serialize_asn1_sequence_TLV_size (serialize_algorithmIdentifier alg) x )
+  | ED25519    -> ( lemma_serialize_asn1_sequence_TLV_size (serialize_algorithmIdentifier alg) x )
+
+let lemma_serialize_algorithmIdentifier_sequence_TLV_size_exact
+  (alg: cryptoAlg {alg == ED25519})
+  (x: algorithmIdentifier_t alg)
+: Lemma (
+  match alg with
+  // | ECDSA_P256 -> ( length_of_opaque_serialization (serialize_algorithmIdentifier_sequence_TLV alg) x == 17 )
+  | ED25519    -> ( lemma_serialize_algorithmIdentifier_size alg x;
+                    length_of_opaque_serialization (serialize_algorithmIdentifier_sequence_TLV alg) x == 7 )
+)
+= match alg with
+  | ED25519    -> ( lemma_serialize_algorithmIdentifier_size alg x;
+                    lemma_serialize_asn1_sequence_TLV_unfold (serialize_algorithmIdentifier alg) x;
+                    lemma_serialize_asn1_sequence_TLV_size   (serialize_algorithmIdentifier alg) x;
+                    // lemma_serialize_algorithmIdentifier_size alg x;
+                    assert_norm (length_of_TLV OID (length_of_opaque_serialization (serialize_algorithmIdentifier alg) x) == 7) )
 
 /// Low
 ///
@@ -195,10 +285,20 @@ let serialize32_algorithmIdentifier_backwards
                     (* g1 *) (synth_algorithmIdentifier_t' alg)
                     (* g1'*) (synth_algorithmIdentifier_t' alg)
                     (* prf*) () )
+  | ED25519    -> ( serialize32_synth_backwards
+                    (* ls *) (serialize32_asn1_TLV_backwards_of_type OID
+                              `serialize32_filter_backwards`
+                              filter_algorithmIdentifier_t' alg)
+                    (* f2 *) (synth_algorithmIdentifier_t alg)
+                    (* g1 *) (synth_algorithmIdentifier_t' alg)
+                    (* g1'*) (synth_algorithmIdentifier_t' alg)
+                    (* prf*) () )
 
 let serialize32_algorithmIdentifier_sequence_TLV_backwards
   (alg: cryptoAlg)
 : serializer32_backwards (serialize_algorithmIdentifier_sequence_TLV alg)
 = match alg with
   | ECDSA_P256 -> ( serialize32_asn1_sequence_TLV_backwards
+                    (* s32 *) (serialize32_algorithmIdentifier_backwards alg) )
+  | ED25519    -> ( serialize32_asn1_sequence_TLV_backwards
                     (* s32 *) (serialize32_algorithmIdentifier_backwards alg) )
