src/asn1/X509.Crypto.fst
@@ -1,3 +1,4 @@
 module X509.Crypto
 
 include X509.Crypto.AlgorithmIdentifier
+include X509.Crypto.Signature
